Move DRBG spec modules to specs/drbg; add interfaces, script and Makefile to generate test vectors

code/drbg/Hacl.HMAC_DRBG.fst
@@ -9,111 +9,36 @@ open Lib.Buffer
 
 module HS = FStar.HyperStack
 module B = LowStar.Buffer
+module LSeq = Lib.Sequence
 
 module HMAC = Hacl.HMAC
 module S = Spec.HMAC_DRBG
-module D = Hacl.Hash.Definitions
-module LSeq = Lib.Sequence
 
-/// HMAC-DRBG
-///
-/// See 10.1.2 and B.2 of
-/// https://nvlpubs.nist.gov/nistpubs/SpecialPublications/NIST.SP.800-90Ar1.pdf
-///
-/// This module implements the hash-algorithm-agile algorithms
-/// - HMAC_DRBG_Update
-/// - HMAC_DRBG_Instantiate_algorithm
-/// - HMAC_DRBG_Reseed_algorithm
-/// - HMAC_DRBG_Generate_algorithm
-///
-/// This is not linked to an appropriate Get_entropy_input function,
-/// so these algorithms should be combined to get entropy from Get_entropy_input
-/// for instantiation, reseeding, and optionally prediction resistance.
-/// 
-/// - Supports SHA-1, SHA2-256, SHA2-384 and SHA2-512 hash algorithms
-///
-/// - Supports reseeding
-/// 
-/// - Supports optional personalization_string for instantiation
-/// 
-/// - Does not support optional additional_input for reseeding or generation
-///
-/// - The internal state is (Key,V,reseed_counter)
-///
-/// - The security_strength is fixed to the HMAC-strength of the hash algorithm
-///   as per p.54 of
-///   https://nvlpubs.nist.gov/nistpubs/SpecialPublications/NIST.SP.800-57pt1r4.pdf
-///
-/// - The minimum entropy for instantiation is 3/2 * security_strength.
-///    - entropy_input must have at least security_strength bits.
-///    - nonce must have at least 1/2 security_strength bits.
-///    - entropy_input and nonce can have at most max_length = 2^16 bits.
-///
-/// - At most max_number_of_bits_per_request = 2^16 bits can be generated per request.
-///
-/// - The reseed_interval is 2^48
-///
-#set-options "--max_fuel 0 --max_ifuel 0 --z3rlimit 50"
+friend Spec.HMAC_DRBG
 
 unfold
-let supported_alg = S.supported_alg
+let hash_len (a:supported_alg) = Hacl.Hash.Definitions.hash_len a
 
-let reseed_interval: n:pub_uint64{v n == S.reseed_interval} = 
-  assert_norm (S.reseed_interval < pow2 64);
-  normalize_term (mk_int S.reseed_interval)
-
-let max_output_length: n:size_t{v n == S.max_output_length} = 
-  assert_norm (S.max_output_length < pow2 32);
-  normalize_term (mk_int S.max_output_length)
-
-let max_length: n:size_t{v n == S.max_length} = 
-  assert_norm (S.max_length < pow2 32);
-  normalize_term (mk_int S.max_length)
-
-let max_personalization_string_length: n:size_t{v n == S.max_personalization_string_length} = 
-  assert_norm (S.max_personalization_string_length < pow2 32);
-  normalize_term (mk_int S.max_personalization_string_length)
-
-let max_additional_input_length: n:size_t{v n == S.max_additional_input_length} = 
-  assert_norm (S.max_additional_input_length < pow2 32);
-  normalize_term (mk_int S.max_additional_input_length)
-
-let min_length (a:supported_alg) : n:size_t{v n == S.min_length a} =
-  assert_norm (S.min_length a < pow2 32);
-  match a with
-  | SHA1 -> normalize_term (mk_int (S.min_length SHA1))
-  | SHA2_256 | SHA2_384 | SHA2_512 -> normalize_term (mk_int (S.min_length SHA2_256))
-
-noeq
-type state (a:hash_alg) =
-| State: 
-    k:lbuffer uint8 (D.hash_len a)
-  -> v:lbuffer uint8 (D.hash_len a)
-  -> reseed_counter:lbuffer pub_uint64 1ul
-    {disjoint k v /\ disjoint k reseed_counter /\ disjoint v reseed_counter}
-  -> state a
-
-let live_st (#a:hash_alg) (h:HS.mem) (st:state a) =
-  let State k v ctr = st in live h k /\ live h v /\ live h ctr
+#set-options "--max_fuel 0 --max_ifuel 0 --z3rlimit 50"
 
 inline_for_extraction noextract
-val update_round: #a:supported_alg 
+val update_round: #a:supported_alg
   -> hmac:HMAC.compute_st a
-  -> len:size_t 
+  -> len:size_t
   -> data:lbuffer uint8 len
   -> n:uint8
-  -> k:lbuffer uint8 (D.hash_len a)
-  -> v:lbuffer uint8 (D.hash_len a)
+  -> k:lbuffer uint8 (hash_len a)
+  -> v:lbuffer uint8 (hash_len a)
   -> ST unit
-  (requires fun h0 -> 
-    live h0 k /\ live h0 v /\ live h0 data /\ 
+  (requires fun h0 ->
+    live h0 k /\ live h0 v /\ live h0 data /\
     disjoint k v /\
     // HMAC input length must fit in size_t
     hash_length a + 1 + uint_v len + block_length a < pow2 32)
   (ensures  fun h0 _ h1 ->
     S.hmac_input_bound a;
-    as_seq h1 k == Spec.Agile.HMAC.hmac a 
-      (as_seq h0 k) 
+    as_seq h1 k == Spec.Agile.HMAC.hmac a
+      (as_seq h0 k)
       (Seq.append (as_seq h0 v) (Seq.cons n (as_seq h0 data))) /\
     as_seq h1 v == Spec.Agile.HMAC.hmac a (as_seq h1 k) (as_seq h0 v) /\
     modifies2 k v h0 h1)
@@ -121,166 +46,128 @@ val update_round: #a:supported_alg
 let update_round #a hmac len data n k v =
   let h0 = get() in
   push_frame();
-  let input_len = D.hash_len a +! 1ul +! len in
+  let input_len = hash_len a +! 1ul +! len in
   let input = create input_len (u8 0) in
-  let k' = sub input 0ul (D.hash_len a) in
+  let k' = sub input 0ul (hash_len a) in
   copy k' v;
-  if len <> 0ul then copy (sub input (D.hash_len a +! 1ul) len) data;
-  input.(D.hash_len a) <- n;
+  if len <> 0ul then copy (sub input (hash_len a +! 1ul) len) data;
+  input.(hash_len a) <- n;
   let h1 = get() in
-  assert (Seq.equal (as_seq h1 input)  
+  assert (Seq.equal (as_seq h1 input)
                     (Seq.append (as_seq h0 v) (Seq.cons n (as_seq h0 data))));
   S.hmac_input_bound a;
-  hmac k' k (D.hash_len a) input input_len;
-  hmac v k' (D.hash_len a) v (D.hash_len a);
+  hmac k' k (hash_len a) input input_len;
+  hmac v k' (hash_len a) v (hash_len a);
   copy k k';
   pop_frame()
 
+
 inline_for_extraction noextract
-val update: #a:supported_alg 
+val update: #a:supported_alg
   -> hmac:HMAC.compute_st a
-  -> len:size_t 
+  -> len:size_t
   -> data:lbuffer uint8 len
-  -> k:lbuffer uint8 (D.hash_len a)
-  -> v:lbuffer uint8 (D.hash_len a)
+  -> k:lbuffer uint8 (hash_len a)
+  -> v:lbuffer uint8 (hash_len a)
   -> ST unit
-  (requires fun h0 -> 
+  (requires fun h0 ->
     live h0 data /\ live h0 k /\ live h0 v /\
     disjoint k v /\ disjoint k data /\ disjoint v data /\
     hash_length a + 1 + uint_v len + block_length a < pow2 32)
   (ensures  fun h0 _ h1 ->
     S.hmac_input_bound a;
-    let k', v' = S.update #a (as_seq h0 data) (as_seq h0 k) (as_seq h0 v) in    
+    let k', v' = S.update #a (as_seq h0 data) (as_seq h0 k) (as_seq h0 v) in
     modifies2 k v h0 h1 /\
     as_seq h1 k == k' /\
     as_seq h1 v == v')
 
 let update #a hmac len data k v  =
   update_round hmac len data (u8 0) k v;
-  if len <> 0ul then 
+  if len <> 0ul then
     update_round hmac len data (u8 1) k v
 
-inline_for_extraction
-let instantiate_st (a:supported_alg) =
-    st:state a 
-  -> entropy_input_len:size_t
-  -> entropy_input:lbuffer uint8 entropy_input_len
-  -> nonce_len:size_t
-  -> nonce:lbuffer uint8 nonce_len
-  -> personalization_string_len:size_t
-  -> personalization_string:lbuffer uint8 personalization_string_len
-  -> ST unit
-  (requires fun h0 -> 
-    live h0 entropy_input /\ live h0 nonce /\ live h0 personalization_string /\
-    live_st h0 st /\
-    S.min_length a <= v entropy_input_len /\ v entropy_input_len <= v max_length /\
-    S.min_length a / 2 <= v nonce_len /\ v nonce_len <= v max_length /\
-    v personalization_string_len <= S.max_personalization_string_length)
-  (ensures  fun h0 _ h1 ->
-    S.hmac_input_bound a;
-    let S.State k v ctr =
-      S.instantiate #a (as_seq h0 entropy_input) (as_seq h0 nonce) 
-        (as_seq h0 personalization_string)
-    in    
-    modifies3 st.k st.v st.reseed_counter h0 h1 /\
-    as_seq h1 st.k == k /\
-    as_seq h1 st.v == v /\
-    uint_v (bget h1 st.reseed_counter 0) == ctr)
+
+noeq
+type state (a:supported_alg) =
+| State:
+    k:lbuffer uint8 (hash_len a)
+  -> v:lbuffer uint8 (hash_len a)
+  -> reseed_counter:lbuffer size_t 1ul
+    {disjoint k v /\ disjoint k reseed_counter /\ disjoint v reseed_counter}
+  -> state a
+
+let footprint #a st =
+  loc st.k |+| loc st.v |+| loc st.reseed_counter
+
+let live_st #a h st =
+  live h st.k /\ live h st.v /\ live h st.reseed_counter
+
+let disjoint_st #a st b =
+  disjoint st.k b /\ disjoint st.v b /\ disjoint st.reseed_counter b
+
+let refl_st #a h st =
+  S.State (as_seq h st.k) (as_seq h st.v) (v (bget h st.reseed_counter 0))
 
 #push-options "--z3rlimit 200"
 
-inline_for_extraction noextract
-val mk_instantiate: #a:supported_alg -> hmac:HMAC.compute_st a -> instantiate_st a
-let mk_instantiate #a hmac st 
-  entropy_input_len entropy_input 
-  nonce_len nonce 
-  personalization_string_len personalization_string 
+let mk_instantiate #a hmac st
+  entropy_input_len entropy_input
+  nonce_len nonce
+  personalization_string_len personalization_string
 =
   let h0 = get () in
   push_frame();
-  let seed_material = create (entropy_input_len +! nonce_len +! personalization_string_len) (u8 0) in  
+  let seed_material = create (entropy_input_len +! nonce_len +! personalization_string_len) (u8 0) in
   copy (sub seed_material 0ul entropy_input_len) entropy_input;
   copy (sub seed_material entropy_input_len nonce_len) nonce;
   copy (sub seed_material (entropy_input_len +! nonce_len) personalization_string_len) personalization_string;
   let State k v ctr = st in
-  fillT (D.hash_len a) k (fun _ -> u8 0) (fun _ -> u8 0);
-  fillT (D.hash_len a) v (fun _ -> u8 1) (fun _ -> u8 1);
+  fillT (hash_len a) k (fun _ -> u8 0) (fun _ -> u8 0);
+  fillT (hash_len a) v (fun _ -> u8 1) (fun _ -> u8 1);
   let h1 = get () in
-  assert (Seq.equal (as_seq h1 seed_material) 
+  assert (Seq.equal (as_seq h1 seed_material)
     (Seq.append (as_seq h0 entropy_input) (Seq.append (as_seq h0 nonce)
       (as_seq h0 personalization_string))));
   assert (LSeq.equal (as_seq h1 k) (LSeq.create (hash_length a) (u8 0)));
   assert (LSeq.equal (as_seq h1 v) (LSeq.create (hash_length a) (u8 1)));
-  ctr.(0ul) <- 1uL;
-  update hmac (entropy_input_len +! nonce_len +! personalization_string_len) 
+  ctr.(0ul) <- 1ul;
+  update hmac (entropy_input_len +! nonce_len +! personalization_string_len)
     seed_material st.k st.v;
   pop_frame()
 
 #pop-options
 
-val instantiate (a:supported_alg) : instantiate_st a
-let instantiate a st 
-  entropy_input_len entropy_input 
+let instantiate a st
+  entropy_input_len entropy_input
   nonce_len nonce
   personalization_string_len personalization_string
 =
   match a with
-  | SHA1     -> 
-    mk_instantiate Hacl.HMAC.legacy_compute_sha1 st 
-      entropy_input_len entropy_input 
+  | SHA1     ->
+    mk_instantiate Hacl.HMAC.legacy_compute_sha1 st
+      entropy_input_len entropy_input
       nonce_len nonce
       personalization_string_len personalization_string
-  | SHA2_256 -> 
+  | SHA2_256 ->
     mk_instantiate Hacl.HMAC.compute_sha2_256 st
-      entropy_input_len entropy_input 
+      entropy_input_len entropy_input
       nonce_len nonce
       personalization_string_len personalization_string
-  | SHA2_384 -> 
+  | SHA2_384 ->
     mk_instantiate Hacl.HMAC.compute_sha2_384 st
-      entropy_input_len entropy_input 
+      entropy_input_len entropy_input
       nonce_len nonce
       personalization_string_len personalization_string
-  | SHA2_512 -> 
+  | SHA2_512 ->
     mk_instantiate Hacl.HMAC.compute_sha2_512 st
-      entropy_input_len entropy_input 
+      entropy_input_len entropy_input
       nonce_len nonce
       personalization_string_len personalization_string
 
 
-inline_for_extraction
-let reseed_st (a:supported_alg) =
-    st:state a 
-  -> entropy_input_len:size_t
-  -> entropy_input:lbuffer uint8 entropy_input_len
-  -> additional_input_len:size_t
-  -> additional_input:lbuffer uint8 additional_input_len
-  -> ST unit
-  (requires fun h0 ->
-    live_st h0 st /\ live h0 entropy_input /\ live h0 additional_input /\
-    disjoint st.k entropy_input /\ disjoint st.v entropy_input /\ 
-    disjoint st.reseed_counter entropy_input /\
-    disjoint st.k additional_input /\ disjoint st.v additional_input /\ 
-    disjoint st.reseed_counter additional_input /\
-    S.min_length a <= v entropy_input_len /\ v entropy_input_len <= v max_length /\
-    v additional_input_len <= S.max_additional_input_length)
-  (ensures  fun h0 _ h1 ->
-    S.hmac_input_bound a;
-    let S.State k v ctr = 
-      S.reseed #a 
-        (S.State (as_seq h0 st.k) (as_seq h0 st.v) (v (bget h0 st.reseed_counter 0)))
-        (as_seq h0 entropy_input)
-        (as_seq h0 additional_input)
-    in
-    modifies3 st.k st.v st.reseed_counter h0 h1 /\
-    as_seq h1 st.k == k /\
-    as_seq h1 st.v == v /\
-    bget h1 st.reseed_counter 0 == 1uL)
-
-inline_for_extraction noextract
-val mk_reseed: #a:supported_alg -> hmac:HMAC.compute_st a -> reseed_st a
-let mk_reseed #a hmac st 
-  entropy_input_len entropy_input 
-  additional_input_len additional_input 
+let mk_reseed #a hmac st
+  entropy_input_len entropy_input
+  additional_input_len additional_input
 =
   let h0 = get () in
   push_frame();
@@ -291,66 +178,33 @@ let mk_reseed #a hmac st
   LSeq.eq_intro (as_seq h1 seed_material)
                 LSeq.(as_seq h0 entropy_input @| as_seq h0 additional_input);
   update hmac (entropy_input_len +! additional_input_len) seed_material st.k st.v;
-  st.reseed_counter.(0ul) <- 1uL;
+  st.reseed_counter.(0ul) <- 1ul;
   pop_frame()
 
-val reseed (a:supported_alg) : reseed_st a
-let reseed a st 
+
+let reseed a st
   entropy_input_len entropy_input
   additional_input_input_len additional_input_input =
   match a with
-  | SHA1 -> 
-    mk_reseed Hacl.HMAC.legacy_compute_sha1 st 
+  | SHA1 ->
+    mk_reseed Hacl.HMAC.legacy_compute_sha1 st
       entropy_input_len entropy_input
       additional_input_input_len additional_input_input
-  | SHA2_256 -> 
-    mk_reseed Hacl.HMAC.compute_sha2_256 st 
+  | SHA2_256 ->
+    mk_reseed Hacl.HMAC.compute_sha2_256 st
       entropy_input_len entropy_input
       additional_input_input_len additional_input_input
-  | SHA2_384 -> 
-    mk_reseed Hacl.HMAC.compute_sha2_384 st 
+  | SHA2_384 ->
+    mk_reseed Hacl.HMAC.compute_sha2_384 st
       entropy_input_len entropy_input
       additional_input_input_len additional_input_input
-  | SHA2_512 -> 
+  | SHA2_512 ->
     mk_reseed Hacl.HMAC.compute_sha2_512 st
       entropy_input_len entropy_input
       additional_input_input_len additional_input_input
 
-
-inline_for_extraction
-let generate_st (a:supported_alg) =
-    output:buffer uint8
-  -> st:state a 
-  -> n:size_t
-  -> additional_input_len:size_t
-  -> additional_input:lbuffer uint8 additional_input_len
-  -> ST bool
-  (requires fun h0 ->
-    live h0 output /\ live_st h0 st /\ live h0 additional_input /\
-    disjoint st.v output /\ disjoint st.k output /\ disjoint st.reseed_counter output /\ disjoint additional_input output /\
-    disjoint st.v additional_input /\ disjoint st.k additional_input /\ disjoint st.reseed_counter additional_input /\
-    v n = length output /\ 
-    0 < v n /\ v n <= S.max_output_length /\
-    v additional_input_len <= S.max_additional_input_length)
-  (ensures  fun h0 b h1 ->
-    S.hmac_input_bound a;
-    let st_ = 
-      S.State (as_seq h0 st.k) (as_seq h0 st.v) (uint_v (bget h0 st.reseed_counter 0)) 
-    in
-    match S.generate #a st_ (v n) (as_seq h0 additional_input) with
-    | None -> b = false /\ modifies0 h0 h1
-    | Some (out, S.State k v ctr) ->
-      b = true /\
-      modifies4 output st.k st.v st.reseed_counter h0 h1 /\
-      as_seq #MUT #_ #n h1 output == out /\
-      as_seq h1 st.k == k /\
-      as_seq h1 st.v == v /\
-      uint_v (bget h1 st.reseed_counter 0) == ctr)
-
 #push-options "--z3rlimit 200"
 
-inline_for_extraction noextract
-val mk_generate: #a:supported_alg -> hmac:HMAC.compute_st a -> generate_st a
 let mk_generate #a hmac output st n additional_input_len additional_input =
   if st.reseed_counter.(0ul) >. reseed_interval then
     false
@@ -361,8 +215,8 @@ let mk_generate #a hmac output st n additional_input_len additional_input =
     if additional_input_len >. 0ul then
       update hmac additional_input_len additional_input st.k st.v;
     let output:lbuffer uint8 n = output in
-    let max = n /. D.hash_len a in
-    let out = sub output 0ul (max *! D.hash_len a) in
+    let max = n /. hash_len a in
+    let out = sub output 0ul (max *! hash_len a) in
     [@inline_let]
     let a_spec = S.a_spec a in
     [@inline_let]
@@ -370,69 +224,61 @@ let mk_generate #a hmac output st n additional_input_len additional_input =
     [@inline_let]
     let spec h0 = S.generate_loop a (as_seq h0 st.k) (v max) in
     let h0 = get () in
-    fill_blocks h0 (D.hash_len a) max out a_spec refl (fun i -> loc st.v) spec 
+    fill_blocks h0 (hash_len a) max out a_spec refl (fun i -> loc st.v) spec
       (fun i ->
-        LSeq.unfold_generate_blocks 
+        LSeq.unfold_generate_blocks
           (hash_length a) (v max) a_spec (spec h0) (as_seq h0 st.v) (v i);
-        hmac st.v st.k (D.hash_len a) st.v (D.hash_len a); 
-        copy (sub out (i *! D.hash_len a) (D.hash_len a)) st.v
+        hmac st.v st.k (hash_len a) st.v (hash_len a);
+        copy (sub out (i *! hash_len a) (hash_len a)) st.v
       );
-    if max *! D.hash_len a <. n then
+    if max *! hash_len a <. n then
       begin
       let h1 = get () in
-      let block = sub output (max *! D.hash_len a) (n -! (max *! D.hash_len a)) in
-      hmac st.v st.k (D.hash_len a) st.v (D.hash_len a);      
-      copy block (sub st.v 0ul (n -! (max *! D.hash_len a)));
+      let block = sub output (max *! hash_len a) (n -! (max *! hash_len a)) in
+      hmac st.v st.k (hash_len a) st.v (hash_len a);
+      copy block (sub st.v 0ul (n -! (max *! hash_len a)));
       let h2 = get () in
-      LSeq.eq_intro (as_seq h2 output) 
+      LSeq.eq_intro (as_seq h2 output)
                     (as_seq h1 out `LSeq.op_At_Bar` as_seq h2 block)
       end;
     update hmac additional_input_len additional_input st.k st.v;
     let ctr = st.reseed_counter.(0ul) in
-    st.reseed_counter.(0ul) <- ctr +! 1uL;
+    st.reseed_counter.(0ul) <- ctr +! 1ul;
     true
     end
 
 #pop-options
 
-val generate (a:supported_alg) : generate_st a
 let generate a output st n additional_input_len additional_input =
   match a with
-  | SHA1     -> 
+  | SHA1     ->
     mk_generate Hacl.HMAC.legacy_compute_sha1 output st n
       additional_input_len additional_input
-  | SHA2_256 -> 
+  | SHA2_256 ->
     mk_generate Hacl.HMAC.compute_sha2_256 output st n
       additional_input_len additional_input
-  | SHA2_384 -> 
+  | SHA2_384 ->
     mk_generate Hacl.HMAC.compute_sha2_384 output st n
       additional_input_len additional_input
-  | SHA2_512 -> 
+  | SHA2_512 ->
     mk_generate Hacl.HMAC.compute_sha2_512 output st n
       additional_input_len additional_input
 
 
-inline_for_extraction noextract
-val alloca_state: a:supported_alg -> StackInline (state a) 
-  (requires fun _ -> True)
-  (ensures  fun h0 st h1 -> 
-    live_st h1 st /\
-    B.modifies B.loc_none h0 h1 /\
-    B.fresh_loc (loc st.k |+| loc st.v |+| loc st.reseed_counter) h0 h1)
 let alloca_state a =
-  let k = 
+  let k =
     match a with
-    | SHA1     -> create (D.hash_len SHA1)     (u8 0)
-    | SHA2_256 -> create (D.hash_len SHA2_256) (u8 0)
-    | SHA2_384 -> create (D.hash_len SHA2_384) (u8 0)
-    | SHA2_512 -> create (D.hash_len SHA2_512) (u8 0)
+    | SHA1     -> create (hash_len SHA1)     (u8 0)
+    | SHA2_256 -> create (hash_len SHA2_256) (u8 0)
+    | SHA2_384 -> create (hash_len SHA2_384) (u8 0)
+    | SHA2_512 -> create (hash_len SHA2_512) (u8 0)
   in
-  let v = 
+  let v =
     match a with
-    | SHA1     -> create (D.hash_len SHA1)     (u8 0)
-    | SHA2_256 -> create (D.hash_len SHA2_256) (u8 0)
-    | SHA2_384 -> create (D.hash_len SHA2_384) (u8 0)
-    | SHA2_512 -> create (D.hash_len SHA2_512) (u8 0)
+    | SHA1     -> create (hash_len SHA1)     (u8 0)
+    | SHA2_256 -> create (hash_len SHA2_256) (u8 0)
+    | SHA2_384 -> create (hash_len SHA2_384) (u8 0)
+    | SHA2_512 -> create (hash_len SHA2_512) (u8 0)
   in
-  let ctr = create 1ul 1uL in
+  let ctr = create 1ul 1ul in
   State k v ctr
