specs/drbg/Spec.HMAC_DRBG.fst
@@ -1,56 +1,33 @@
 module Spec.HMAC_DRBG
 
-open Spec.Hash.Definitions
-open Spec.Agile.HMAC
-
 open Lib.IntTypes
 open FStar.Seq
 open FStar.Mul
 
-/// HMAC-DRBG
-///
-/// See 10.1.2 in
-/// https://nvlpubs.nist.gov/nistpubs/SpecialPublications/NIST.SP.800-90Ar1.pdf
-/// 
+open Spec.Hash.Definitions
+open Spec.Agile.HMAC
 
 #set-options "--max_fuel 0 --max_ifuel 0 --z3rlimit 50"
 
-let supported_alg = a:hash_alg{ is_supported_alg a }
-
-let reseed_interval   = pow2 48
-let max_output_length = pow2 16
-let max_length        = pow2 16
-let max_personalization_string_length = pow2 16
-let max_additional_input_length = pow2 16
-
-/// See p.54
-/// https://nvlpubs.nist.gov/nistpubs/SpecialPublications/NIST.SP.800-57pt1r4.pdf
-let min_length (a:supported_alg) =
-  match a with
-  | SHA1 -> 16
-  | SHA2_256 | SHA2_384 | SHA2_512 -> 32
-
 noeq
 type state (a:supported_alg) =
-| State: 
-    k:lbytes (hash_length a) 
-  -> v:lbytes (hash_length a) 
+| State:
+    k:lbytes (hash_length a)
+  -> v:lbytes (hash_length a)
   -> reseed_counter:nat
   -> state a
 
-val hmac_input_bound: a:supported_alg -> Lemma 
-  (hash_length a + pow2 32 + pow2 32 + 1 + block_length a + block_length a <= max_input_length a)
 let hmac_input_bound = function
-  | SHA1     -> 
+  | SHA1     ->
     let a = SHA1 in
     assert_norm (hash_length a + pow2 32 + pow2 32 +1 + block_length a + block_length a <= max_input_length a)
-  | SHA2_256 ->   
+  | SHA2_256 ->
     let a = SHA2_256 in
     assert_norm (hash_length a + pow2 32 + pow2 32 + 1 + block_length a + block_length a <= max_input_length a)
-  | SHA2_384 -> 
+  | SHA2_384 ->
     let a = SHA2_384 in
     assert_norm (hash_length a + pow2 32 + pow2 32 + 1 + block_length a + block_length a <= max_input_length a)
-  | SHA2_512 -> 
+  | SHA2_512 ->
     let a = SHA2_512 in
     assert_norm (hash_length a + pow2 32 + pow2 32 + 1 + block_length a + block_length a <= max_input_length a)
 
@@ -61,6 +38,7 @@ val update: #a:supported_alg
   -> Pure (lbytes (hash_length a) & lbytes (hash_length a))
   (requires hash_length a + Seq.length data + 1 + block_length a <= max_input_length a)
   (ensures  fun _ -> True)
+
 let update #a data k v =
   let zero_data = Seq.cons (u8 0) data in
   let k = hmac a k (v @| zero_data) in
@@ -71,39 +49,15 @@ let update #a data k v =
     let one_data = Seq.cons (u8 1) data in
     let k = hmac a k (v @| one_data) in
     let v = hmac a k v in
-    k, v 
+    k, v
 
-(* We omit personalization_string *)
-val instantiate: #a:supported_alg
-  -> entropy_input:bytes
-  -> nonce:bytes
-  -> personalization_string:bytes
-  -> Pure (state a)
-  (requires
-    hash_length a
-    + Seq.length entropy_input 
-    + Seq.length nonce 
-    + Seq.length personalization_string 
-    + 1 + block_length a <= max_input_length a)
-  (ensures fun _ -> True)
 let instantiate #a entropy_input nonce personalization_string =
   let seed_material = entropy_input @| nonce @| personalization_string in
   let k = Seq.create (hash_length a) (u8 0) in
-  let v = Seq.create (hash_length a) (u8 1) in  
+  let v = Seq.create (hash_length a) (u8 1) in
   let k, v = update #a seed_material k v in
   State k v 1
 
-val reseed: #a:supported_alg
-  -> state a
-  -> entropy_input: bytes
-  -> additional_input: bytes
-  -> Pure (state a)
-  (requires 
-    hash_length a + 
-    Seq.length entropy_input + 
-    Seq.length additional_input +
-    1 + block_length a <= max_input_length a)
-  (ensures fun _ -> True)
 let reseed #a st entropy_input additional_input =
   let seed_material = entropy_input @| additional_input in
   let k, v = update #a seed_material st.k st.v in
@@ -124,22 +78,13 @@ let generate_loop a k max i vi =
   hmac_input_bound a;
   let v = hmac a k vi in v, v
 
-(* We omit additional_input; n is the number of **bytes** requested *)
-val generate: #a:supported_alg
-  -> state a
-  -> n:pos{n <= max_output_length}
-  -> additional_input: bytes
-  -> Pure (option (lbytes n & state a))
-  (requires hash_length a + Seq.length additional_input + 1 + block_length a <= max_input_length a)
-  (ensures fun _ -> True)
 let generate #a st n additional_input =
-  hmac_input_bound a;
-  if st.reseed_counter > reseed_interval then 
+  if st.reseed_counter > reseed_interval then
     None
   else
-    let k, v = 
-      if Seq.length additional_input > 0 then
-        update additional_input st.k st.v 
+    let k, v =
+      if Seq.length additional_input > 0 then 
+        update additional_input st.k st.v
       else st.k, st.v
     in
     let max = n / hash_length a in
@@ -161,19 +106,22 @@ let generate #a st n additional_input =
 (** Equivalently, but proving it requires proving extensionality of generate_blocks *)
 val generate': #a:supported_alg
   -> state a
-  -> n:pos{n <= max_output_length}
-  -> additional_input: bytes
+  -> n:nat
+  -> additional_input:bytes
   -> Pure (option (lbytes n & state a))
-  (requires hash_length a + Seq.length additional_input + 1 + block_length a <= max_input_length a)
+  (requires
+    0 < n /\ n <= max_output_length /\
+    hash_length a + Seq.length additional_input
+      + 1 + block_length a <= max_input_length a)
   (ensures fun _ -> True)
 let generate' #a st n additional_input =
   hmac_input_bound a;
-  if st.reseed_counter > reseed_interval then 
+  if st.reseed_counter > reseed_interval then
     None
-  else    
-    let k, v = 
+  else
+    let k, v =
       if Seq.length additional_input > 0 then
-        update additional_input st.k st.v 
+        update additional_input st.k st.v
       else st.k, st.v
     in
     // let max = ceil (n / hash_length a) in
