specs/tests/Spec.HMAC_DRBG.Test.fst
@@ -5,7 +5,7 @@ open Lib.IntTypes
 
 open Spec.Agile.HMAC
 open Spec.HMAC_DRBG
-open Spec.HMAC_DRBG.Vectors
+open Spec.HMAC_DRBG.Test.Vectors
 
 #set-options "--max_fuel 1 --max_ifuel 1 --z3rlimit 50"
 
@@ -22,7 +22,7 @@ let rec as_uint8s acc
 
 #pop-options
 
-let from_hex (s:hex_string) : lseq uint8 (String.strlen s / 2) = 
+let from_hex (s:hex_string) : lseq uint8 (String.strlen s / 2) =
   seq_of_list (as_uint8s [] (String.list_of_string s))
 
 let print_and_compare (len:size_nat) (test_expected test_result:lbytes len) : All.ML bool =
@@ -34,10 +34,10 @@ let print_and_compare (len:size_nat) (test_expected test_result:lbytes len) : Al
   List.iter (fun a -> IO.print_uint8_hex_pad a) (seq_to_list test_expected);
   Lib.ByteSequence.lbytes_eq #len test_expected test_result
 
-let test_vec 
-  {a; entropy_input; entropy_input_reseed; nonce; personalization_string;   
+let test_vec
+  {a; entropy_input; entropy_input_reseed; nonce; personalization_string;
    additional_input_reseed; additional_input_1; additional_input_2;
-   returned_bits} 
+   returned_bits}
 =
   let returned_bytes_len       = String.strlen returned_bits / 2 in
   let entropy_input_len        = String.strlen entropy_input / 2 in
@@ -46,19 +46,19 @@ let test_vec
   let personalization_string_len = String.strlen personalization_string / 2 in
   let additional_input_reseed_len = String.strlen additional_input_reseed / 2 in
   let additional_input_1_len   = String.strlen additional_input_1 / 2 in
-  let additional_input_2_len   = String.strlen additional_input_2 / 2 in  
+  let additional_input_2_len   = String.strlen additional_input_2 / 2 in
   let returned_bits_len        = String.strlen returned_bits / 2 in
   if not (is_supported_alg a &&
-          min_length a <= entropy_input_len && 
+          min_length a <= entropy_input_len &&
           entropy_input_len <= max_length &&
-          min_length a / 2 <= nonce_len && 
+          min_length a / 2 <= nonce_len &&
           nonce_len <= max_length &&
           personalization_string_len <= max_personalization_string_length &&
           entropy_input_reseed_len <= max_length &&
           additional_input_reseed_len <= max_additional_input_length &&
           additional_input_1_len <= max_additional_input_length &&
           additional_input_2_len <= max_additional_input_length &&
-          0 < returned_bits_len && 
+          0 < returned_bits_len &&
           returned_bits_len <= max_output_length)
   then false
   else
@@ -66,25 +66,25 @@ let test_vec
     let st = instantiate #a
       (from_hex entropy_input) (from_hex nonce) (from_hex personalization_string)
     in
-    let st = reseed st 
-      (from_hex entropy_input_reseed) (from_hex additional_input_reseed) 
+    let st = reseed st
+      (from_hex entropy_input_reseed) (from_hex additional_input_reseed)
     in
     match generate st returned_bytes_len (from_hex additional_input_1) with
     | None -> false
-    | Some (_, st) -> 
+    | Some (_, st) ->
       match generate st returned_bytes_len (from_hex additional_input_2) with
       | None -> false
       | Some (out, st) -> print_and_compare returned_bytes_len (from_hex returned_bits) out
 
 let test () =
   let result = List.for_all test_vec test_vectors in
-  if result then 
-    begin 
-    IO.print_string "\n\n[HMAC-DRBG] PASS\n"; 
-    true 
+  if result then
+    begin
+    IO.print_string "\n\n[HMAC-DRBG] PASS\n";
+    true
     end
-  else 
-    begin 
-    IO.print_string "\n\n[HMAC-DRBG] FAIL\n"; 
-    false 
+  else
+    begin
+    IO.print_string "\n\n[HMAC-DRBG] FAIL\n";
+    false
     end
